extra/MoreSemantics.v
@@ -1,0 +1,79 @@
+    [pat_bool : bool -> pat
+  | pat_int : int -> pat
+
+
+
+
+(** Evaluation rules for pattern matching. 
+    [patmatch v p] returns:
+    - [None] if the value [v] is not an instance of the pattern [p],
+    - [Some S] is the value [v] is equal to the instantiation of [p]
+      with the bindings from [S]. *)
+
+Definition patmatch (v:val) (p:pat) : option ctx :=
+  (* If (exists G, patsubst G p = v) then Some (epsilon such G) else None *)
+  match p, v with
+  | pat_var x, _ => Some (Ctx.one_var x v)
+  | pat_constr id1 xs, val_constr id2 vs => 
+      If id1 = id2 /\ length xs = length vs /\ var_distinct xs
+        then Some (Ctx.combine xs vs)
+        else None
+  | _, _ => None
+  end.
+
+
+
+
+
+Lemma map_lookup_combine : forall `{Inhab A} xs vs (E:ctx A),
+  E = combine xs vs ->
+  length xs = length vs ->
+  var_distinct xs ->
+  LibList.map (fun x => lookup_or_arbitrary x E) xs = vs.
+Proof using.
+  introv HE HL HD. gen E HD.
+  unfold combine. rewrite~ List_combine_eq.
+  list2_ind~ xs vs. clears xs vs. (* LATER: automate clear? *)
+  intros x1 xs1 x2 xs2 EQ IH E HE HD.
+  rew_listx in *. (* LATER bug does not perform [rewrite map_cons] *)
+  rew_listx. fequals. 
+  { subst E. rewrite~ lookup_or_arbitrary_cons_same. }
+  { destruct HD as (HN&HD'). sets_eq E': (LibList.combine xs1 xs2). subst E.
+    rewrites* <- (>> IH E'). applys map_congr.
+    { intros x Hx. rewrite~ lookup_or_arbitrary_cons_neq.
+      forwards*: var_fresh_mem_inv HN Hx. } }
+Qed.
+
+
+
+(* ********************************************************************** *)
+(* * Correctness of pattern matching evaluation/instantiation *)
+
+Lemma patmatch_inv_patsubst : forall v p Gopt,
+  patmatch v p = Gopt ->
+  match Gopt with
+  | None => forall G, v <> patsubst G p
+  | Some G => v = patsubst G p
+  end.
+Proof using.
+  introv E. induction p; simpl.
+  { subst Gopt. simpl. unfold Ctx.one_var, Ctx.lookup_or_arbitrary, Ctx.lookup.
+    rewrite var_eq_spec. case_if*. (* LATER: lemma *) }
+  { destruct Gopt as [G|].
+    { destruct v; tryfalse.
+      { simpls. case_if as C. destruct C as (C1&C2&C3). subst. 
+        inverts E. rewrites~ (>> Ctx.map_lookup_combine C2). } }
+    { intros G N. destruct v; tryfalse.
+      { inverts N. simpls. case_if as C. false C. rew_listx~. } } }
+Qed.
+
+Lemma patmatch_eq_None_inv : forall v p,
+  patmatch v p = None -> 
+  forall G, v <> patsubst G p.
+Proof using. introv H. applys (>> patmatch_inv_patsubst H). Qed.
+
+Lemma patmatch_eq_Some_inv : forall v p G,
+  patmatch v p = Some G -> 
+  v = patsubst G p.
+Proof using. introv H. applys (>> patmatch_inv_patsubst H). Qed.
+
